the correctness instance for CPS translation (L4_5 to L5)

certicoq/theories/L4_deBruijn/instances.v
@@ -70,7 +70,7 @@ Proof.
     pose proof (L3_to_L4_correct.translate_correct e t).
     eexists.
     constructor. apply H2.
-Admitted. 
+Admitted.
 
 Global Instance certiL3_to_L4_correct :
   CerticoqTranslationCorrect certiL3 certiL4.
@@ -99,6 +99,7 @@ Proof.
       intros. constructor. }
 Qed.
 
+
 Require Import L4.L4_5_to_L5.
 Require Import SquiggleEq.export.
 Require Import SquiggleEq.UsefulTypes.
@@ -110,15 +111,27 @@ Global  Program Instance : BigStepOpSem L4_5_Term L4_5_Term := eval.
 
 (** all variables must be user variables *)
 Global Program Instance : GoodTerm L4_5_Term :=
-  fun e  => varsOfClass (all_vars e) true /\ isprogram e.
+  fun e  => varsOfClass (all_vars e) true /\ isprogram e /\ fixwf e = true.
 
-(* FIX!! *)
+Require Import DecidableClass.
 Global Instance QuestionHeadTermL45 : QuestionHead (prod ienv L4_5_Term) :=
-fun q t => false.
+fun q t =>
+match q, snd t with
+| Cnstr ind ci, oterm (NDCon dc _) _ =>
+  let (ind2, ci2) := dc in
+  andb (decide (ind=ind2)) (decide (N.of_nat ci =ci2))
+| Abs, oterm NLambda _ => true
+| _, _ => false
+end.
 
-(* FIX!! *)
 Global Instance ObsSubtermTermL45 : ObserveNthSubterm (prod ienv L4_5_Term) :=
-fun n t => None.
+  fun n t =>
+    let (env, t) := t in
+    match t with
+    | oterm (NDCon dc _) lbt =>
+      List.nth_error  (List.map (fun b => (env, get_nt b)) lbt) n
+    | _ => None
+    end.
 
 Global Instance certiL4_5: CerticoqLanguage (prod ienv L4_5_Term) := {}.
 
@@ -127,49 +140,162 @@ Global Instance certiL4_to_L4_5:
   CerticoqTotalTranslation (cTerm certiL4) (cTerm certiL4_5) :=
   fun p => (fst p, (L4_2_to_L4_5 (tL4_to_L4_2 (snd p))) ).
 
+  
+
+
 Require Import L4.variables.
 
 Definition L5Term :Type := (@NTerm NVar L5Opid).
 
 Global Program Instance : BigStepOpSem L5Term L5Term := eval_c.
 
-Global Program Instance : GoodTerm L5Term := isprogram.
+(* may need to strengthened: consider adding the predicated nt_wf and fixwf.
+It seems that there is currently there is no proof that cps_cvt nt_wf.
+A more direct alternative to nt_wf could be the predicate that says that the conversion from
+L5 to L5a succeeds.  *)
+Global Program Instance : GoodTerm L5Term := closed (*isprogram *).
 
-(* FIX!! *)
 Global Instance QuestionHeadTermL5 : QuestionHead (ienv * L5Term) :=
-fun q t => false.
+fun q t =>
+match q, snd t with
+| Cnstr ind ci, oterm (CDCon dc _) _ =>
+  let (ind2, ci2) := dc in
+  andb (decide (ind=ind2)) (decide (N.of_nat ci =ci2))
+| Abs, oterm CLambda _ => true
+| _, _ => false
+end.
 
-(* FIX!! *)
 Global Instance ObsSubtermTermL5 : ObserveNthSubterm (ienv * L5Term) :=
-fun n t => None.
+  fun n t =>
+    let (env, t) := t in
+    match t with
+    | oterm (CDCon dc _) lbt =>
+      List.nth_error  (List.map (fun b => (env, get_nt b)) lbt) n
+    | _ => None
+    end.
 
 Global Instance certiL5: CerticoqLanguage (ienv * L5Term) := {}.
 
+Definition haltCont : L5Term := KLam_c contVar (Halt_c (vterm contVar)).
+
+Lemma haltContAp t : eval_c (Ret_c haltCont t) t.
+Proof.
+  unfold haltCont.
+  rewrite eval_ret.
+  simpl. unfold subst. simpl.
+  apply eval_Halt_c.
+Qed.
+
 Global Instance certiL4_5_to_L5:
   CerticoqTotalTranslation (cTerm certiL4_5) (cTerm certiL5):=
-  (fun x => (fst x,  (cps_cvt (snd x)))).
+  (fun x => (fst x, Ret_c (cps_cvt (snd x)) haltCont)).
+
+Definition oldTranslation : (cTerm certiL4_5) -> (cTerm certiL5):=
+  (fun x => (fst x, (cps_cvt (snd x)))).
+
+Require Import SquiggleEq.tactics.
+
+(* Move to L4_5_to_L5 *)
+Hint Unfold isprogram : eval.
+Hint Resolve @eval_yields_value' @eval_preseves_varclass 
+  @eval_preseves_wf @eval_preserves_closed conj
+  @cps_cvt_val_closed @cps_cvt_closed @eval_preserves_fixwf @eval_end: eval.
+
+Require Import Btauto.
+Lemma valueObsEq (senv: ienv) : forall (sv:L4_5_Term), is_value sv ->
+                                                  (senv, sv) ⊑ (senv, cps_cvt_val sv).
+Proof using.
+  intros ? Hisv.
+  induction Hisv; simpl.
+- constructor; compute; intros qn; [ destruct qn | ]; constructor.
+- constructor; compute; intros qn; [ destruct qn | ]; constructor.
+- constructor.
+  + unfold yesPreserved, questionHead, QuestionHeadTermL45, QuestionHeadTermL5; cbn.
+    destruct q; auto. unfold implb. btauto.
+  + clear H. rename H0 into Hind. intros ?. cbn. repeat rewrite List.map_map.
+    repeat rewrite  list.nth_error_map.
+    remember (List.nth_error es n) as esso.
+    destruct esso as [ess | ]; try constructor.
+    simpl. apply Hind.
+    eapply List.nth_error_In.
+    symmetry. eassumption.
+- constructor; compute; intros qn; [ destruct qn | ]; try constructor.
+Qed.
+                                                  
+Require Import L4.variables.
+Require Import L4.varInterface.
+Global Instance certiL4_5_to_L5Correct: CerticoqTranslationCorrect certiL4_5 certiL5.
+Proof.
+  constructor.
+- simpl. red. intros ? Hgood.
+  unfold certiClasses.translate, liftTotal, bigStepEval,
+  liftBigStepException, translateT, certiL4_5_to_L5. simpl.
+  simpl. hnf. simpl.
+  unfold goodTerm, dummyEnvWf, goodTerm, GoodTerm_instance_0, isprogram, closed in Hgood.
+  destruct s as [? s]; simpl in *. repnd.
+  hnf. simpl. symmetry. rewrite cps_cvt_aux_fvars; auto. rewrite Hgood2. refl.
+- red. intros ? ? Hgood Heval.
+  destruct Heval as [Heq Heval].
+  destruct s as [senv s].
+  destruct sv as [? sv]. symmetry in Heq.
+  simpl in *. subst.
+  exists (senv, (cps_cvt_val sv)).
+  unfold certiClasses.translate, liftTotal, bigStepEval,
+  liftBigStepException, translateT, certiL4_5_to_L5. simpl.
+  repeat progress (unfold bigStepEval, dummyEnvBigStep; simpl).
+  unfold BigStepOpSem_instance_1. simpl.
+  simpl. unfold bigStepEval, dummyEnvBigStep. simpl.
+  unfold goodTerm, dummyEnvWf, goodTerm, GoodTerm_instance_0 in Hgood.
+  simpl in *. repnd. destruct Hgood1 as [Hclosed Hwf].
+  rename Hgood0 into Hvc. rename Hgood into Hfixwf.
+  dands;[reflexivity | | ].
+  + pose proof
+         (cps_cvt_corr _ _ Hwf Hfixwf Hvc Heval
+                       Hclosed haltCont
+                       eq_refl
+                       ((cps_cvt_val sv)))
+      as Hcps.
+    apply Hcps. clear Hcps.
+    hnf in Heval.
+    rewrite (cps_val_ret_flip sv); try split; eauto with eval typeclass_instances.
+    unfold haltCont.
+    apply haltContAp.
+    
+  + hnf in Heval. apply eval_yields_value' in Heval.
+    revert Heval. clear.
+    apply valueObsEq.
+Qed.
+
 
 Require Import L4.L5a.
 
 (* Fix. Define subst and evaluation on L5a by going to L5 via a bijection? *)
-Global Program Instance : BigStepOpSem L4.L5a.val_c  L4.L5a.val_c :=
+Global Program Instance : BigStepOpSem L4.L5a.cps  L4.L5a.cps :=
   fun _ _ => True.
 
 (** Fix *)
-Global Program Instance : GoodTerm L4.L5a.val_c := fun x => False.
+Global Program Instance : GoodTerm L4.L5a.cps := fun x => False.
 
 (* FIX!! *)
-Global Instance QuestionHeadTermL5a : QuestionHead (ienv * L4.L5a.val_c) :=
+Global Instance QuestionHeadTermL5a : QuestionHead (ienv * L4.L5a.cps) :=
 fun q t => false.
 
 (* FIX!! *)
-Global Instance ObsSubtermTermL5a: ObserveNthSubterm (ienv * L4.L5a.val_c) :=
+Global Instance ObsSubtermTermL5a: ObserveNthSubterm (ienv * L4.L5a.cps) :=
 fun n t => None.
 
-Global Instance certiL5a: CerticoqLanguage (ienv * L4.L5a.val_c) := {}.
+Global Instance certiL5a: CerticoqLanguage (ienv * L4.L5a.cps) := {}.
 
 Global Instance certiL5_to_L5a: 
   CerticoqTranslation (cTerm certiL5) (cTerm certiL5a)  :=
+  fun e =>
+   match L4.L5a.translateCPS (snd e) with
+  | None => exceptionMonad.Exc "error in L5a.translateVal"
+  | Some e5a => exceptionMonad.Ret (fst e, e5a)
+  end.
+
+Definition certiL5_to_L5aOld : 
+  CerticoqTranslation (cTerm certiL5) (ienv * L4.L5a.val_c)  :=
   fun e =>
    match L4.L5a.translateVal (snd e) with
   | None => exceptionMonad.Exc "error in L5a.translateVal"
@@ -221,13 +347,43 @@ match e with
 | Exc s => Exc s
 end.
 
+(*
+Require Import L1g.instances.
+Require Import L2.instances.
+Require Import L2_5.instances.
+Require Import L2.instances.
+  
 
-(***
-Eval vm_compute in (exception_map print4 (ctranslateTo certiL4_2 p0L1)).
-Eval vm_compute in (exception_map print5 (ctranslateTo certiL5 p0L1)).
-Eval vm_compute in ( (ctranslateTo certiL5 p0L1)).
+Quote Recursively Definition v0L1 := 0. 
+  
+Definition v0L45 := Eval vm_compute in ( (ctranslateTo certiL4_5 v0L1)).
+Print v0L45.
+Definition p0L5New := Eval vm_compute in (exception_map certiL4_5_to_L5 v0L45).
+Definition p0L5Old := Eval vm_compute in (exception_map oldTranslation v0L45).
+
+
+Eval compute in (exception_map print5 p0L5New).
+Eval compute in (exception_map print5 p0L5Old).
+
+Eval compute in (exception_map snd (bind p0L5New certiL5_to_L5a)).
+(*
+Ret
+         (Ret_c
+            (Cont_c (3%positive, nNamed "k")
+               (Ret_c (KVar_c (3%positive, nNamed "k"))
+                  (Con_c (mkInd "Coq.Init.Datatypes.nat" 0, 0%N) [])))
+            (Cont_c (3%positive, nNamed "k") (Halt_c (KVar_c (3%positive, nNamed "k")))))
+ *)
+Eval compute in (exception_map snd (bind p0L5Old certiL5_to_L5aOld)).
+
+(*
+(Cont_c (3%positive, nNamed "k")
+            (Ret_c (KVar_c (3%positive, nNamed "k"))
+               (Con_c (mkInd "Coq.Init.Datatypes.nat" 0, 0%N) [])))
+*)
 
 Quote Recursively Definition evo := (andb (even 0) (odd 1)).
+
 Eval vm_compute in (exception_map print4 (ctranslateTo certiL4_2 evo)).
 Eval vm_compute in (exception_map print5 (ctranslateTo certiL5 evo)).
 
@@ -245,15 +401,4 @@ Check  @cps_cvt_corr.
            (Ret_c (KVar_c 5%positive) (Con_c (mkInd "Coq.Init.Datatypes.nat" 0, 0%N) nil)))
      : exception (cTerm certiL5a)
 *)
-
-
-  
-
-
-
-
-
-
-
-
 
